\documentclass{article}
\usepackage[utf8]{inputenc}
\usepackage{setspace}
\usepackage{amsmath}
\usepackage{amsthm}
\usepackage{amsfonts}
\usepackage{amssymb}
\usepackage{natbib}
\usepackage{graphicx}
\usepackage[dvipsnames]{xcolor}
\graphicspath{ {./images/} }
\usepackage[legalpaper, portrait, margin=0.9in]{geometry}
\title{ASSIGNMENT 6}
\author{Neeraj Pandey}
\date{Discrete Mathematics}


\begin{document}


\maketitle
\begin{flushleft}
\textbf{Q1: } Prove that $4^n + n^4$ is not a prime for $n > 1$.
\newline
\newline
\textbf{Solution: } \begin{itemize}

    \item If n is even, then the equation is even: \[4^n + n^4 = 4^2x + (2x)^ 4 \in 2x = n \]
        Therefore, it is not even
    \item if n is odd, $n = 2x + 1$,
    \[= 4^n + n^4\]
    \[= 4^{(2x +1)} + n^4\]
    \[= 4^{(2x)}\cdot4 + n^4\]
    \[= 4{(2^x)}^{4} + n^4 \]
    \[= {(2{(2^x)}^2)^2} + {4n^{2}{(2^x)}^2} - {4n^2{(2^x)}^2}\]
    \[= {(n^2 + 2 \cdot {(2^x)})^2} - {(2n \cdot 2^x)^2}\]
    \[= {(n^2 + 2 \cdot {(2^x)} + (2n \cdot 2^x)) } \cdot {(n^2 + 2 \cdot {(2^x)} - (2n \cdot 2^x)) }\]
    \[= {((n + 2^x)^2 + 4^x) \cdot ((n - 2^x)^2 + 4^k)}\]
    When n is odd, the equation $4^n + n^4$ is not prime because it can be expressed as a product of more than two factors and 2 or more than 2 are greater than 1.
    \newline
    Hence, proved.

\end{itemize}

\end{flushleft}



\begin{flushleft}
\textbf{Q2: } Let $a, b, c, d$ are integers such that $a \neq c$. Suppose $a - c | ab + c d$. Is it true that $a âˆ’ c | ad + b c$? Justify your answer.
\newline
\newline
\newcommand\tab[1][1cm]{\hspace*{#1}}
\textbf{Solution: } From the given details, \[(a - c)x = ab + c d \tab[0.2cm]for\tab[0.2cm] x\in Z  \]
\[= (a b + c d) - (a d + b c)\]
\[= a b + c d - a d - b c  \]
\[= a(b - d) + c(b - d)\]
\[= (a - c)\cdot(b - d)\]
\[\implies (a b + c d) - (a d + b c) =  (a - c)\cdot(b - d)\]
\[(a d + b c) =  (a b +  c d) - ((a - c)\cdot(b - d))\]
\[(a d + b c) =  (a - c)x - ((a - c)\cdot(b - d))\]
\[\implies (a d + b c) = (a - c)\cdot(x - b + d) \]

By Closure property, $a - c | ab + c d$.
hence, proved.



\end{flushleft}


\end{document}
